replace `List` in `Envs` with new `Env`

src/Iris/Proofmode/Environments.lean
@@ -4,21 +4,91 @@ namespace Iris.Proofmode
 open Iris.BI
 open Lean
 
-structure Envs (PROP : Type) [BI PROP] where
-  intuitionistic : List PROP
-  spatial : List PROP
+-- Env
+inductive Env (α : Type)
+  | nil  : Env α
+  | cons : α → Env α → Env α
 
-def of_envs [BI PROP] (Γₚ Γₛ : List PROP) : PROP :=
+namespace Env
+
+@[reducible]
+def concat : Env α → α → Env α
+  | .nil, b       => .cons b .nil
+  | .cons a as, b => .cons a <| as.concat b
+
+@[reducible]
+def isEmpty : Env α → Bool
+  | .nil      => true
+  | .cons _ _ => false
+
+@[reducible]
+def length : Env α → Nat
+  | .nil       => 0
+  | .cons _ as => as.length + 1
+
+@[reducible]
+def eraseIdx : (e : Env α) → Fin (e.length) → Env α
+  | .cons _ as, ⟨0    , _⟩ => as
+  | .cons a as, ⟨i + 1, h⟩ => .cons a <| as.eraseIdx ⟨i, Nat.le_of_succ_le_succ h⟩
+
+@[reducible]
+def get : (e : Env α) → Fin (e.length) → α
+  | .cons a _ , ⟨0    , _⟩ => a
+  | .cons _ as, ⟨i + 1, h⟩ => as.get ⟨i, Nat.le_of_succ_le_succ h⟩
+
+@[reducible]
+def partition (as : Env α) (mask : List Bool) : Env α × Env α :=
+  go as mask
+where
+  @[reducible]
+  go : Env α → List Bool → Env α × Env α
+  | .cons a as, b :: bs =>
+    let (ls, rs) := go as bs
+    if b then
+      (.cons a ls, rs)
+    else
+      (ls, .cons a rs)
+  | _, _ =>
+    (.nil, nil)
+
+@[reducible]
+def toList : Env α → List α
+  | .nil       => []
+  | .cons a as => a :: toList as
+
+inductive Mem : α → Env α → Prop
+  | head (a : α) (as : Env α)         : Mem a (.cons a as)
+  | tail (a : α) (as : Env α) {b : α} : Mem b as → Mem b (.cons a as)
+
+instance : Membership α (Env α) where
+  mem := Mem
+
+instance : Coe (Env α) (List α) where
+  coe := toList
+
+instance [ToString α] : ToString <| Env α where
+  toString e := e.toList.toString
+
+end Env
+
+
+-- Envs
+structure Envs (PROP : Type) [BI PROP] where
+  intuitionistic : Env PROP
+  spatial        : Env PROP
+
+def of_envs [BI PROP] (Γₚ Γₛ : Env PROP) : PROP :=
   match Γₚ, Γₛ with
-  | [], [] => `[iprop| emp]
-  | _, []  => `[iprop| □ [∧] Γₚ]
-  | [], _  => `[iprop| [∗] Γₛ]
-  | _, _   => `[iprop| □ [∧] Γₚ ∗ [∗] Γₛ]
+  | .nil, .nil => `[iprop| emp]
+  | _   , .nil => `[iprop| □ [∧] Γₚ]
+  | .nil, _    => `[iprop| [∗] Γₛ]
+  | _   , _    => `[iprop| □ [∧] Γₚ ∗ [∗] Γₛ]
 
 def envs_entails [BI PROP] (Δ : Envs PROP) (Q : PROP) : Prop :=
   of_envs Δ.intuitionistic Δ.spatial ⊢ Q
 
 
+-- HypothesisIndex
 inductive HypothesisType | intuitionistic | spatial
 
 structure HypothesisIndex where
@@ -37,22 +107,23 @@ def HypothesisIndex.quoteAsEnvsIndex : HypothesisIndex → MetaM Syntax
     `(EnvsIndex.s ⟨$(quote index), by show $(quote index) < $(quote length) ; decide⟩)
 
 
-class AffineEnv [BI PROP] (Γ : List PROP) where
-  affineEnv : ∀ p, p ∈ Γ → Affine p
+-- AffineEnv
+class AffineEnv [BI PROP] (Γ : Env PROP) where
+  affineEnv : ∀ P, P ∈ Γ → Affine P
 
 instance affineEnvNil [BI PROP] :
-  AffineEnv (PROP := PROP) []
+  AffineEnv (PROP := PROP) .nil
 where
   affineEnv := sorry
 
-instance affineEnvCons [BI PROP] (P : PROP) (Γ : List PROP) :
+instance affineEnvConcat [BI PROP] (P : PROP) (Γ : Env PROP) :
   [Affine P] →
   [AffineEnv Γ] →
-  AffineEnv (P :: Γ)
+  AffineEnv (.cons P Γ)
 where
   affineEnv := sorry
 
-instance (priority := default + 10) affineEnvBi [BIAffine PROP] (Γ : List PROP) :
+instance (priority := default + 10) affineEnvBi [BIAffine PROP] (Γ : Env PROP) :
   AffineEnv Γ
 where
   affineEnv := sorry
