src/Iris/Proofmode/Expr.lean
@@ -4,7 +4,7 @@ import Iris.Std.Expr
 
 namespace Iris.Proofmode
 open Iris.BI
-open Lean Lean.Expr
+open Lean Lean.Expr Lean.Meta
 
 def isEmp (expr : Expr) : Bool := expr.isAppOfArity ``BIBase.emp 2
 
@@ -31,4 +31,82 @@ def modifyEnvsEntails? (expr : Expr) (Γₚ Γₛ P : Option Expr) : Option Expr
   let expr := modifyAppOptM expr #[none, none, envs, P]
   some expr
 
+
+namespace EnvExpr
+
+partial def any? (env : Expr) (pred : Expr → Bool) : MetaM <| Option Bool := do
+  let env ← whnf env
+  if let some (_, a, env') := app3? env ``Env.cons then
+    if pred a then return true
+    else any? env' pred
+  else if let some _ := app1? env ``Env.nil then
+    return false
+  else
+    return none
+
+partial def findIndexM? [Monad M] [MonadLift MetaM M] (env : Expr) (pred : Expr → M Bool) : M <| Option Nat :=
+  go env 0
+where
+  go (env : Expr) (idx : Nat) : M <| Option Nat := do
+    let env ← whnf env
+    if let some (_, a, env') := app3? env ``Env.cons then
+      if ← pred a then pure <| some idx
+      else go env' (idx + 1)
+    else
+      pure none
+
+partial def findIndex? (env : Expr) (pred : Expr → Bool) : MetaM <| Option Nat := do
+  have : MonadLift MetaM MetaM := { monadLift := id }
+  findIndexM? env (return pred ·)
+
+def get? (env : Expr) (i : Nat) : MetaM <| Option Expr := do
+  let env ← whnf env
+  match i with
+  | 0 =>
+    if let some (_, a, _) := app3? env ``Env.cons then
+      return a
+    else
+      return none
+  | i + 1 =>
+    if let some (_, _, env') := app3? env ``Env.cons then
+      get? env' i
+    else
+      return none
+
+partial def length? (env : Expr) : MetaM <| Option Nat :=
+  go env 0
+where
+  go (env : Expr) (length : Nat) : MetaM <| Option Nat := do
+    let env ← whnf env
+    if let some (_, _, env') := app3? env ``Env.cons then
+      go env' (length + 1)
+    else if let some _ := app1? env ``Env.nil then
+      return length
+    else
+      return none
+
+def set? (env : Expr) (e : Expr) (i : Nat) : MetaM <| Option Expr := do
+  let env ← whnf env
+  match i with
+  | 0 => do
+    let some _ := app3? env ``Env.cons
+      | pure none
+    return modifyAppOptM env #[none, e, none]
+  | i + 1 => do
+    let some (_, _, env') := app3? env ``Env.cons
+      | pure none
+    let some env' ← set? env' e i
+      | pure none
+    return modifyAppOptM env #[none, none, env']
+
+partial def toEnv? (env : Expr) : MetaM <| Option <| Env Expr := do
+  let env ← whnf env
+  if let some (_, a, env') := app3? env ``Env.cons then
+    return (← toEnv? env') |>.map (.cons a ·)
+  else if let some _ := app1? env ``Env.nil then
+    return some .nil
+  else
+    return none
+
+end EnvExpr
 end Iris.Proofmode
