src/Iris/Proofmode/Theorems.lean
@@ -1,7 +1,6 @@
 import Iris.BI
 import Iris.Proofmode.Classes
 import Iris.Proofmode.Environments
-import Iris.Std.List
 import Iris.Std.TC
 
 namespace Iris.Proofmode
@@ -9,29 +8,29 @@ open Iris.BI Iris.Std
 
 -- proof mode
 theorem tac_start [BI PROP] (P : PROP) :
-  envs_entails ⟨[], []⟩ P →
+  envs_entails ⟨.nil, .nil⟩ P →
   ⊢ P
 := sorry
 
-theorem tac_clear [BI PROP] {Γₚ Γₛ : List PROP} (i : EnvsIndex Γₚ.length Γₛ.length) (Q : PROP) :
+theorem tac_clear [BI PROP] {Γₚ Γₛ : Env PROP} (i : EnvsIndex Γₚ.length Γₛ.length) (Q : PROP) :
   let (p, P, Γₚ', Γₛ') := match i with
-    | .p i => (true, Γₚ.getR i, Γₚ.eraseIdxR i, Γₛ)
-    | .s i => (false, Γₛ.getR i, Γₚ, Γₛ.eraseIdxR i)
+    | .p i => (true, Γₚ.get i, Γₚ.eraseIdx i, Γₛ)
+    | .s i => (false, Γₛ.get i, Γₚ, Γₛ.eraseIdx i)
   [TCIte p TCTrue (TCOr (Affine P) (Absorbing Q))] →
   envs_entails ⟨Γₚ', Γₛ'⟩ Q →
   envs_entails ⟨Γₚ, Γₛ⟩ Q
 := sorry
 
 -- implication and wand
-theorem tac_impl_intro [BI PROP] {Γₚ Γₛ : List PROP} {P Q : PROP} (R : PROP) :
+theorem tac_impl_intro [BI PROP] {Γₚ Γₛ : Env PROP} {P Q : PROP} (R : PROP) :
   [FromImpl R P Q] →
-  [TCIte Γₛ.isEmptyR TCTrue (Persistent P)] →
+  [TCIte Γₛ.isEmpty TCTrue (Persistent P)] →
   [FromAffinely P' P] →
   envs_entails ⟨Γₚ, Γₛ.concat P'⟩ Q →
   envs_entails ⟨Γₚ, Γₛ⟩ R
 := sorry
 
-theorem tac_impl_intro_intuitionistic [BI PROP] {Γₚ Γₛ : List PROP} {P P' Q : PROP} (R : PROP) :
+theorem tac_impl_intro_intuitionistic [BI PROP] {Γₚ Γₛ : Env PROP} {P P' Q : PROP} (R : PROP) :
   [FromImpl R P Q] →
   [IntoPersistent false P P'] →
   envs_entails ⟨Γₚ.concat P', Γₛ⟩ Q →
@@ -44,13 +43,13 @@ theorem tac_impl_intro_drop [BI PROP] {Δ : Envs PROP} {P Q : PROP} (R : PROP) :
   envs_entails Δ R
 := sorry
 
-theorem tac_wand_intro [BI PROP] {Γₚ Γₛ : List PROP} {P Q : PROP} (R : PROP) :
+theorem tac_wand_intro [BI PROP] {Γₚ Γₛ : Env PROP} {P Q : PROP} (R : PROP) :
   [FromWand R P Q] →
   envs_entails ⟨Γₚ, Γₛ.concat P⟩ Q →
   envs_entails ⟨Γₚ, Γₛ⟩ R
 := sorry
 
-theorem tac_wand_intro_intuitionistic [BI PROP] {Γₚ Γₛ : List PROP} {P P' Q : PROP} (R : PROP) :
+theorem tac_wand_intro_intuitionistic [BI PROP] {Γₚ Γₛ : Env PROP} {P P' Q : PROP} (R : PROP) :
   [FromWand R P Q] →
   [IntoPersistent false P P'] →
   [TCOr (Affine P) (Absorbing Q)] →
@@ -65,67 +64,67 @@ theorem tac_forall_intro [BI PROP] {Δ : Envs PROP} {Ψ : α → PROP} (Q : PROP
 := sorry
 
 -- assumptions
-theorem tac_assumption_lean [BI PROP] {Γₚ Γₛ : List PROP} {P : PROP} (Q : PROP) :
+theorem tac_assumption_lean [BI PROP] {Γₚ Γₛ : Env PROP} {P : PROP} (Q : PROP) :
   (⊢ P) →
   [FromAssumption true P Q] →
-  [TCIte Γₛ.isEmptyR TCTrue (TCOr (Absorbing Q) (AffineEnv Γₛ))] →
+  [TCIte Γₛ.isEmpty TCTrue (TCOr (Absorbing Q) (AffineEnv Γₛ))] →
   envs_entails ⟨Γₚ, Γₛ⟩ Q
 := sorry
 
-theorem tac_assumption [BI PROP] {Γₚ Γₛ : List PROP} (i : EnvsIndex Γₚ.length Γₛ.length) (Q : PROP) :
+theorem tac_assumption [BI PROP] {Γₚ Γₛ : Env PROP} (i : EnvsIndex Γₚ.length Γₛ.length) (Q : PROP) :
   let (p, P) := match i with
-    | .p i => (true, Γₚ.getR i)
-    | .s i => (false, Γₛ.getR i)
+    | .p i => (true, Γₚ.get i)
+    | .s i => (false, Γₛ.get i)
   [FromAssumption p P Q] →
-  let Γₛ' := if let .s i := i then Γₛ.eraseIdxR i else Γₛ
-  [TCIte Γₛ'.isEmptyR TCTrue (TCOr (Absorbing Q) (AffineEnv Γₛ'))] →
+  let Γₛ' := if let .s i := i then Γₛ.eraseIdx i else Γₛ
+  [TCIte Γₛ'.isEmpty TCTrue (TCOr (Absorbing Q) (AffineEnv Γₛ'))] →
   envs_entails ⟨Γₚ, Γₛ⟩ Q
 := sorry
 
 -- false
-theorem tac_false_destruct [BI PROP] {Γₚ Γₛ : List PROP} (i : EnvsIndex Γₚ.length Γₛ.length) (Q : PROP) :
+theorem tac_false_destruct [BI PROP] {Γₚ Γₛ : Env PROP} (i : EnvsIndex Γₚ.length Γₛ.length) (Q : PROP) :
   let P := match i with
-    | .p i => Γₚ.getR i
-    | .s i => Γₛ.getR i
+    | .p i => Γₚ.get i
+    | .s i => Γₛ.get i
   P = `[iprop| False] →
   envs_entails ⟨Γₚ, Γₛ⟩ Q
 := sorry
 
 -- moving between contexts
-theorem tac_pure [BI PROP] {Γₚ Γₛ : List PROP} {φ : Prop} (i : EnvsIndex Γₚ.length Γₛ.length) (Q : PROP) :
+theorem tac_pure [BI PROP] {Γₚ Γₛ : Env PROP} {φ : Prop} (i : EnvsIndex Γₚ.length Γₛ.length) (Q : PROP) :
    let (p, P) := match i with
-    | .p i => (true, Γₚ.getR i)
-    | .s i => (false, Γₛ.getR i)
+    | .p i => (true, Γₚ.get i)
+    | .s i => (false, Γₛ.get i)
   [IntoPure P φ] →
   [TCIte p TCTrue (TCOr (Affine P) (Absorbing Q))] →
    let (Γₚ', Γₛ') := match i with
-    | .p i => (Γₚ.eraseIdxR i, Γₛ)
-    | .s i => (Γₚ, Γₛ.eraseIdxR i)
+    | .p i => (Γₚ.eraseIdx i, Γₛ)
+    | .s i => (Γₚ, Γₛ.eraseIdx i)
   (φ → envs_entails ⟨Γₚ', Γₛ'⟩ Q) →
   envs_entails ⟨Γₚ, Γₛ⟩ Q
 := sorry
 
-theorem tac_intuitionistic [BI PROP] {Γₚ Γₛ : List PROP} {P' : PROP} (i : EnvsIndex Γₚ.length Γₛ.length) (Q : PROP) :
+theorem tac_intuitionistic [BI PROP] {Γₚ Γₛ : Env PROP} {P' : PROP} (i : EnvsIndex Γₚ.length Γₛ.length) (Q : PROP) :
   let (p, P) := match i with
-    | .p i => (true, Γₚ.getR i)
-    | .s i => (false, Γₛ.getR i)
+    | .p i => (true, Γₚ.get i)
+    | .s i => (false, Γₛ.get i)
   [IntoPersistent p P P'] →
   [TCIte p TCTrue (TCOr (Affine P) (Absorbing Q))] →
   let (Γₚ', Γₛ') := match i with
-    | .p i => (Γₚ |>.eraseIdxR i |>.concat P', Γₛ)
-    | .s i => (Γₚ.concat P', Γₛ.eraseIdxR i)
+    | .p i => (Γₚ |>.eraseIdx i |>.concat P', Γₛ)
+    | .s i => (Γₚ.concat P', Γₛ.eraseIdx i)
   envs_entails ⟨Γₚ', Γₛ'⟩ Q →
   envs_entails ⟨Γₚ, Γₛ⟩ Q
 := sorry
 
-theorem tac_spatial [BI PROP] {Γₚ Γₛ : List PROP} {P' : PROP} (i : EnvsIndex Γₚ.length Γₛ.length) (Q : PROP) :
+theorem tac_spatial [BI PROP] {Γₚ Γₛ : Env PROP} {P' : PROP} (i : EnvsIndex Γₚ.length Γₛ.length) (Q : PROP) :
   let (p, P) := match i with
-    | .p i => (true, Γₚ.getR i)
-    | .s i => (false, Γₛ.getR i)
+    | .p i => (true, Γₚ.get i)
+    | .s i => (false, Γₛ.get i)
   [FromAffinely P' P p] →
   let (Γₚ', Γₛ') := match i with
-    | .p i => (Γₚ.eraseIdxR i, Γₛ.concat P')
-    | .s i => (Γₚ, Γₛ |>.eraseIdxR i |>.concat P')
+    | .p i => (Γₚ.eraseIdx i, Γₛ.concat P')
+    | .s i => (Γₚ, Γₛ |>.eraseIdx i |>.concat P')
   envs_entails ⟨Γₚ', Γₛ'⟩ Q →
   envs_entails ⟨Γₚ, Γₛ⟩ Q
 := sorry
@@ -138,10 +137,9 @@ theorem tac_and_split [BI PROP] {Δ : Envs PROP} {Q1 Q2 : PROP} (P : PROP) :
   envs_entails Δ P
 := sorry
 
-theorem tac_sep_split [BI PROP] {Γₚ Γₛ : List PROP} {Q1 Q2 : PROP} (sortedIndices : List Nat) (splitRight : Bool) (P : PROP) :
+theorem tac_sep_split [BI PROP] {Γₚ Γₛ : Env PROP} {Q1 Q2 : PROP} (mask : List Bool) (P : PROP) :
   [FromSep P Q1 Q2] →
-  let (Γₛ₁, Γₛ₂) := Γₛ.partitionIndices (sortedIndices.contains ·)
-  let (Γₛ₁, Γₛ₂) := if splitRight then (Γₛ₂, Γₛ₁) else (Γₛ₁, Γₛ₂)
+  let (Γₛ₁, Γₛ₂) := Γₛ.partition mask
   envs_entails ⟨Γₚ, Γₛ₁⟩ Q1 →
   envs_entails ⟨Γₚ, Γₛ₂⟩ Q2 →
   envs_entails ⟨Γₚ, Γₛ⟩ P
@@ -155,43 +153,43 @@ class inductive IntoConjunction [BI PROP] (P : PROP) (P1 P2 : outParam PROP) : B
 attribute [instance] IntoConjunction.and
 attribute [instance] IntoConjunction.sep
 
-theorem tac_conjunction_destruct [BI PROP] {Γₚ Γₛ : List PROP} {P1 P2 : PROP} (i : EnvsIndex Γₚ.length Γₛ.length) (Q : PROP) :
+theorem tac_conjunction_destruct [BI PROP] {Γₚ Γₛ : Env PROP} {P1 P2 : PROP} (i : EnvsIndex Γₚ.length Γₛ.length) (Q : PROP) :
   let (p, P) := match i with
-    | .p i => (true, Γₚ.getR i)
-    | .s i => (false, Γₛ.getR i)
+    | .p i => (true, Γₚ.get i)
+    | .s i => (false, Γₛ.get i)
   [IntoConjunction P P1 P2 p] →
   let (Γₚ', Γₛ') := match i with
-    | .p i => (Γₚ |>.eraseIdxR i |>.concat P1 |>.concat P2, Γₛ)
-    | .s i => (Γₚ, Γₛ |>.eraseIdxR i |>.concat P1 |>.concat P2)
+    | .p i => (Γₚ |>.eraseIdx i |>.concat P1 |>.concat P2, Γₛ)
+    | .s i => (Γₚ, Γₛ |>.eraseIdx i |>.concat P1 |>.concat P2)
   envs_entails ⟨Γₚ', Γₛ'⟩ Q →
   envs_entails ⟨Γₚ, Γₛ⟩ Q
 := sorry
 
-theorem tac_conjunction_destruct_choice [BI PROP] {Γₚ Γₛ : List PROP} {P1 P2 : PROP} (i : EnvsIndex Γₚ.length Γₛ.length) (d : Bool) (Q : PROP) :
+theorem tac_conjunction_destruct_choice [BI PROP] {Γₚ Γₛ : Env PROP} {P1 P2 : PROP} (i : EnvsIndex Γₚ.length Γₛ.length) (d : Bool) (Q : PROP) :
   let (p, P) := match i with
-    | .p i => (true, Γₚ.getR i)
-    | .s i => (false, Γₛ.getR i)
+    | .p i => (true, Γₚ.get i)
+    | .s i => (false, Γₛ.get i)
   [IntoAnd p P P1 P2] →
   let P' := if d then P1 else P2
   let (Γₚ', Γₛ') := match i with
-    | .p i => (Γₚ |>.eraseIdxR i |>.concat P', Γₛ)
-    | .s i => (Γₚ, Γₛ |>.eraseIdxR i |>.concat P')
+    | .p i => (Γₚ |>.eraseIdx i |>.concat P', Γₛ)
+    | .s i => (Γₚ, Γₛ |>.eraseIdx i |>.concat P')
   envs_entails ⟨Γₚ', Γₛ'⟩ Q →
   envs_entails ⟨Γₚ, Γₛ⟩ Q
 := sorry
 
-theorem tac_disjunction_destruct [BI PROP] {Γₚ Γₛ : List PROP} {P1 P2 : PROP} (i : EnvsIndex Γₚ.length Γₛ.length) (Q : PROP) :
+theorem tac_disjunction_destruct [BI PROP] {Γₚ Γₛ : Env PROP} {P1 P2 : PROP} (i : EnvsIndex Γₚ.length Γₛ.length) (Q : PROP) :
   let P := match i with
-    | .p i => Γₚ.getR i
-    | .s i => Γₛ.getR i
+    | .p i => Γₚ.get i
+    | .s i => Γₛ.get i
   [IntoOr P P1 P2] →
   let (Γₚₗ, Γₚᵣ, Γₛₗ, Γₛᵣ) := match i with
     | .p i => (
-      Γₚ |>.eraseIdxR i |>.concat P1, Γₚ |>.eraseIdxR i |>.concat P2,
+      Γₚ |>.eraseIdx i |>.concat P1, Γₚ |>.eraseIdx i |>.concat P2,
       Γₛ, Γₛ)
     | .s i => (
       Γₚ, Γₚ,
-      Γₛ |>.eraseIdxR i |>.concat P1, Γₛ |>.eraseIdxR i |>.concat P2)
+      Γₛ |>.eraseIdx i |>.concat P1, Γₛ |>.eraseIdx i |>.concat P2)
   envs_entails ⟨Γₚₗ, Γₛₗ⟩ Q →
   envs_entails ⟨Γₚᵣ, Γₛᵣ⟩ Q →
   envs_entails ⟨Γₚ, Γₛ⟩ Q
