src/Iris/Std/List.lean
@@ -1,15 +1,5 @@
 namespace List
 
-@[reducible]
-def isEmptyR : List α → Bool
-  | []     => true
-  | _ :: _ => false
-
-@[reducible]
-def eraseIdxR : (as : List α) → Fin as.length → List α
-  | _ :: as, ⟨0, _⟩     => as
-  | a :: as, ⟨i + 1, h⟩ => a :: eraseIdxR as ⟨i, Nat.le_of_succ_le_succ h⟩
-
 @[specialize]
 def foldl1 {α} (f : α → α → α) (alt : Unit → α) : List α → α
   | []     => alt ()
@@ -20,24 +10,5 @@ def foldr1 {α} (f : α → α → α) (alt : Unit → α) : List α → α
   | []     => alt ()
   | [a]    => a
   | a :: l => f a (foldr1 f alt l)
-
-@[reducible]
-def getR : (as : List α) → Fin as.length → α
-  | a :: _ , ⟨0, _⟩     => a
-  | _ :: as, ⟨i + 1, h⟩ => getR as ⟨i, Nat.le_of_succ_le_succ h⟩
-
-@[specialize]
-def partitionIndices (as : List α) (p : Nat → Bool) : List α × List α :=
-  go as 0
-where
-  go (as : List α) (idx : Nat) : List α × List α :=
-    match as with
-    | []      => ([], [])
-    | a :: as =>
-      let as' := go as (idx + 1)
-      if p idx then
-        as'.map (a :: ·) (·)
-      else
-        as'.map (·) (a :: ·)
 
 end List
